L1.v
@@ -2,27 +2,27 @@ Require Import DataTypes Omega Coq.Logic.Classical MsiState.
 
 Module Type L1Axioms (dt: DataTypes).
   Import dt.
-  Axiom deqOrNot: forall t, {x| deqR (fst x) (snd x) t} + {forall c i, ~ deqR c i t}.
-  Axiom deqLeaf: forall {c i t}, deqR c i t -> leaf c.
-  Axiom deqDef: forall {c i t}, deqR c i t -> defined c.
-  Axiom uniqDeqProc: forall {c i1 t i2},
-                       deqR c i1 t -> deqR c i2 t ->
+  Axiom deqOrNot: forall a t, {x| deqR a (fst x) (snd x) t} + {forall c i, ~ deqR a c i t}.
+  Axiom deqLeaf: forall {c a i t}, deqR a c i t -> leaf c.
+  Axiom deqDef: forall {c a i t}, deqR a c i t -> defined c.
+  Axiom uniqDeqProc: forall {c a i1 t i2},
+                       deqR a c i1 t -> deqR a c i2 t ->
                        i1 = i2.
-  Axiom uniqDeqProc2: forall {c i t1 t2},
-                        deqR c i t1 -> deqR c i t2 -> t1 = t2.
-  Axiom uniqDeqProc3: forall {c1 i1 t c2 i2},
-                       deqR c1 i1 t -> deqR c2 i2 t ->
+  Axiom uniqDeqProc2: forall {c a i t1 t2},
+                        deqR a c i t1 -> deqR a c i t2 -> t1 = t2.
+  Axiom uniqDeqProc3: forall {c1 a i1 t c2 i2},
+                       deqR a c1 i1 t -> deqR a c2 i2 t ->
                        c1 = c2 /\ i1 = i2.
-  Axiom deqOrder: forall {c i1 t1 i2 t2},
-                    deqR c i1 t1 -> deqR c i2 t2 ->
+  Axiom deqOrder: forall {c a i1 t1 i2 t2},
+                    deqR a c i1 t1 -> deqR a c i2 t2 ->
                     i1 < i2 -> ~ t1 > t2.
-  Axiom processDeq: forall {c i t}, deqR c i t -> let q := reqFn c i in
+  Axiom processDeq: forall {c a i t}, deqR a c i t -> let q := reqFn a c i in
                                           match desc q with
-                                            | Ld => sle Sh (state c (loc q) t)
-                                            | St => state c (loc q) t = Mo
+                                            | Ld => sle Sh (state c a t)
+                                            | St => state c a t = Mo
                                           end.
-  Parameter deqImpDeqBefore: forall {c i1 i2 t},
-                               deqR c i1 t -> i2 < i1 -> exists t', t' < t /\ deqR c i2 t'.
+  Parameter deqImpDeqBefore: forall {c a i1 i2 t},
+                               deqR a c i1 t -> i2 < i1 -> exists t', t' < t /\ deqR a c i2 t'.
 End L1Axioms.
 
 Module Type L1Theorems (dt: DataTypes) (l1A: L1Axioms dt).
@@ -35,22 +35,21 @@ Module Type L1Theorems (dt: DataTypes) (l1A: L1Axioms dt).
     (data c a t = initData a /\
      forall {ti}, 0 <= ti < t -> forall {ci ii},
                                    defined ci ->
-                                   ~ (deqR ci ii ti /\ loc (reqFn ci ii) = a /\
-                                      desc (reqFn ci ii) = St)) \/
-    (exists cb ib tb, defined cb /\ tb < t /\ deqR cb ib tb /\ desc (reqFn cb ib) = St /\
-                      loc (reqFn cb ib) = a /\
-                      data c a t = dataQ (reqFn cb ib) /\
+                                   ~ (deqR a ci ii ti /\
+                                      desc (reqFn a ci ii) = St)) \/
+    (exists cb ib tb, defined cb /\ tb < t /\ deqR a cb ib tb /\ desc (reqFn a cb ib) = St /\
+                      data c a t = dataQ (reqFn a cb ib) /\
                       forall {ti}, tb < ti < t ->
                                    forall {ci ii},
                                      defined ci ->
-                                     ~ (deqR ci ii ti /\ loc (reqFn ci ii) = a /\
-                                        desc (reqFn ci ii) = St)
+                                     ~ (deqR a ci ii ti /\
+                                        desc (reqFn a ci ii) = St)
     ).
 
   Parameter uniqM:
   forall {c a t}, defined c -> leaf c ->
     state c a t = Mo -> forall {co}, defined co -> leaf co -> c <> co -> state co a t = In.
 
-  Parameter deqOrNot: forall t, {x| deqR (fst x) (snd x) t} + {forall c i, ~ deqR c i t}.
+  Parameter deqOrNot: forall a t, {x| deqR a (fst x) (snd x) t} + {forall c i, ~ deqR a c i t}.
 
 End L1Theorems.
